update jitfix

theory/JITFix.thy
@@ -1,135 +1,8 @@
 theory JITFix
-  imports JITFlattern
+  imports JITFix_aux
 begin
 
-value "x64_encode (Pcall_i 0x1111)"
 
-value "u8_list_of_i32 0x1111"
-
-value "x64_encode (Pjcc Cond_e 0x00000000)"
-
-value "u8_list_of_i32 0x11110000"
-
-value "u32_of_u8_list [0,0,0,0]"
-
-fun x64_bin_update ::"nat \<Rightarrow> x64_bin \<Rightarrow> nat \<Rightarrow> u8 list \<Rightarrow> x64_bin " where
-  "x64_bin_update 0 l _ _ = l" |
-  "x64_bin_update (Suc n) l pc u8_list =  (let l' = list_update l pc (hd u8_list) in x64_bin_update n l' (pc+1) (tl u8_list))"
-
-value "x64_bin_update 4 [232::8 word, 0::8 word, 0::8 word, 0::8 word, 0::8 word] 1 [17::8 word, 17::8 word, 0::8 word, 0::8 word]"
-
-value "x64_bin_update 4 [15::8 word, 132::8 word, 0::8 word, 0::8 word, 17::8 word, 17::8 word] 2 [0::8 word, 0::8 word, 17::8 word, 17::8 word]"
-
-definition get_updated_l_bin::"(int\<times>u64) \<Rightarrow> x64_bin \<Rightarrow> (int \<times> nat) list \<Rightarrow> x64_bin option"where
-  "get_updated_l_bin x l l_pc \<equiv> 
-    (let fix_begin_addr = fst (l_pc!(nat(fst x))); 
-        (target_begin_addr,num2) = l_pc!(unat (snd x)) in 
-        (case x64_decode (nat fix_begin_addr) l of 
-              Some(sz, Pcall_i _) \<Rightarrow> let offset = ((of_int target_begin_addr)::i32) - ((of_int fix_begin_addr+of_nat sz+1)::i32) in 
-                                     let u8_list = x64_encode (Pcall_i (ucast offset)) in
-                                     Some (x64_bin_update (length u8_list) l (nat fix_begin_addr) u8_list) |
-              Some(sz, Pcmpq_rr src dst) \<Rightarrow> let loc = nat fix_begin_addr+sz in 
-                    (case x64_decode loc l of 
-                            Some(sz2, Pjcc cond _) \<Rightarrow> let offset = ((of_int target_begin_addr)::i32) - ((of_nat (loc+sz2)+1)::i32) in
-                                                      let u8_list = x64_encode (Pjcc cond (ucast offset)) in                                                     
-                                                      Some (x64_bin_update (length u8_list) l loc u8_list) | 
-                            _ \<Rightarrow> None ) |
-              _ \<Rightarrow> None ))"
-
-
-value "x64_decode 0 [72::8 word, 57::8 word, 195::8 word] "
-
-
-value "x64_decode 0 [15::8 word, 132::8 word, 0::8 word, 0::8 word, 0::8 word, 0::8 word] "
-
-
-value "get_updated_l_bin (0,1) [72::8 word, 57::8 word, 195::8 word, 15::8 word, 132::8 word, 0::8 word, 0::8 word, 0::8 word, 0::8 word ,195::8 word] [(0::int, 8::nat), (9::int, 1::nat)]"
-
-value "get_updated_l_bin (0,1) [232::8 word, 0::8 word, 0::8 word, 0::8 word, 0::8 word ,195::8 word] [(0::int, 1::nat), (6::int, 1::nat)]"
-
-(*input: l_jump x64_bin l_pc*)
-fun jitfix :: "((int\<times>u64) list) \<Rightarrow> x64_bin \<Rightarrow> (int \<times> nat) list \<Rightarrow> x64_bin option" where
-  "jitfix [] l _  = Some l" |
-  "jitfix (x#xs) l l_pc = (if l = [] then None else 
-    let res = get_updated_l_bin x l l_pc in case res of None \<Rightarrow> None | 
-                                                        Some l' \<Rightarrow> jitfix xs l' l_pc)"
-
-value "x64_encode (Pcmpq_rr RAX RBX)"
-
-value "x64_encode (Pret)"
-
-value "jitflat_bpf [(1, 1, [0x48,0x01,0xD8]),(1, 2, [0x48, 0x39, 0xc3, 0x0f, 0x84, 0x00, 0x00, 0x00, 0x00]), (1, 1, [0x48,0x01,0xD8]), (1, 1, [0x48,0x01,0xD8])] init_second_layer"
-
-value "jitfix [(1::int, 3::64 word)] [72::8 word, 1::8 word, 216::8 word, 72::8 word, 57::8 word, 195::8 word, 15::8 word, 132::8 word, 0::8 word, 0::8 word, 0::8 word, 0::8 word, 72::8 word, 1::8 word, 216::8 word, 72::8 word, 1::8 word, 216::8 word] [(0::int, 1::nat), (3::int, 1::nat), (12::int, 1::nat), (15::int, 1::nat)]"
-
-value "jitflat_bpf [(1, 2, [0x48, 0x39, 0xc3, 0x0f, 0x84, 0x00, 0x00, 0x00, 0x00]), (1, 1, [0xc3]), (1, 1, [0x48,0x01,0xD8]), (1, 1, [0x48,0x01,0xD8]),(1, -3, [0x48, 0x39, 0xc3, 0x0f, 0x84, 0x00, 0x00, 0x00, 0x00])] init_second_layer"
-
-value "jitfix [(0::int, 2::64 word), (4::int, 1::64 word)] [72::8 word, 57::8 word, 195::8 word, 15::8 word, 132::8 word, 0::8 word, 0::8 word, 0::8 word, 0::8 word, 195::8 word, 72::8 word, 1::8 word, 216::8 word, 72::8 word, 1::8 word, 216::8 word, 72::8 word, 57::8 word, 195::8 word,
-   15::8 word, 132::8 word, 0::8 word, 0::8 word, 0::8 word, 0::8 word] [(0::int, 1::nat), (9::int, 1::nat), (10::int, 1::nat), (13::int, 1::nat), (16::int, 1::nat)]"
-
-(*
-
-definition x64_bin_update ::"x64_bin \<Rightarrow> nat \<Rightarrow> u8 list \<Rightarrow> x64_bin " where
- "x64_bin_update l pc u8_list \<equiv>  ( let l1 = list_update l pc (u8_list!0);
-                                       l2 = list_update l1 (pc+1) (u8_list!1);
-                                       l3 = list_update l2 (pc+2) (u8_list!2);   
-                                       l4 = list_update l3 (pc+3) (u8_list!3) in l4)"
-
-definition get_updated_l_bin::"(int\<times>u64) \<Rightarrow> x64_bin \<Rightarrow> (int \<times> nat) list \<Rightarrow> x64_bin"where
-  "get_updated_l_bin x l l_pc \<equiv> 
-    (let fix_begin_addr = fst (l_pc!(nat(fst x))); 
-        (target_begin_addr,num2) = l_pc!(unat (snd x)) in 
-        (case x64_decode (nat fix_begin_addr) l of 
-              Some(_, Pcall_i _) \<Rightarrow> let offset = ((of_int target_begin_addr)::i32) - ((of_int fix_begin_addr+5+1)::i32);
-                              u8_list = u8_list_of_i32 offset in
-                              x64_bin_update l (nat (fix_begin_addr+1)) u8_list | 
-              _ \<Rightarrow> let offset = ((of_int target_begin_addr)::i32) - ((of_int fix_begin_addr+3+6+1)::i32);
-                              u8_list = u8_list_of_i32 offset in                                                     
-                             x64_bin_update l (nat (fix_begin_addr+3+2)) u8_list))"*)
-
-
-
-(*definition update_l_jump_further::"flat_bpf_prog \<Rightarrow> hybrid_state \<Rightarrow> (hybrid_state \<times> flat_bpf_prog)" where
- "update_l_jump_further lp st = (
-  let (l_bin,l_pc,l_jump) = lp in
-  let (pc, xst) = st in
-    (case xst of
-    Stuck \<Rightarrow> ((pc, Stuck), lp) |
-    Next xpc rs m ss \<Rightarrow> (
-    if unat pc \<ge> length l_pc \<or> unat pc < 0 then ((pc, Stuck), lp) else 
-    let num = snd (l_pc!(unat pc)) in 
-    let old_xpc = nat (fst (l_pc!(unat pc))) in 
-      if xpc \<noteq> old_xpc then ((pc, Stuck), lp) else 
-        if (\<exists> d. x64_decode xpc l_bin = Some(5, Pcall_i d)) then
-            (case find_target_pc_in_l_pc l_jump (uint pc) of 
-              None \<Rightarrow> ((pc, Stuck), lp) |
-              Some npc \<Rightarrow> 
-                (let caller = save_x64_caller rs; fp = save_x64_frame_pointer rs; 
-                    rs' = upate_x64_stack_pointer rs (stack_pointer ss) in
-                let ss' = update_stack caller fp (pc+1) ss in
-                  (case ss' of None \<Rightarrow> ((pc, Stuck), lp) | 
-                  Some ra \<Rightarrow> ((npc, (Next (nat (fst (l_pc!(unat npc)))) rs' m ra)), lp))))
-        else if (\<exists> src dst. x64_decode xpc l_bin = Some(3, Pcmpq_rr src dst)) then \<comment>\<open> TODO: if the first byte is the opcode of cmp? \<close>
-          \<comment>\<open> case: BPF JMP \<close>
-          (case x64_sem num l_bin (Next xpc rs m ss) of
-          Stuck \<Rightarrow> ((pc, Stuck), lp) | \<comment>\<open> if one step error, stop, it should be impossible \<close>
-          Next xpc1 rs1 m1 ss1 \<Rightarrow> (
-            if rs1 (CR ZF) = 1 then \<comment>\<open> must JUMP \<close>
-              (case find_target_pc_in_l_pc l_jump (uint pc) of
-              None \<Rightarrow> ((pc, Stuck), lp) |
-              Some npc \<Rightarrow>
-                ((npc, (Next (nat (fst (l_pc!(unat npc)))) rs1 m1 ss1)),lp)) \<comment>\<open> go to the target address in the jited x64 binary \<close>
-            else \<comment>\<open> donot JUMP \<close>
-              ((pc+1, (Next xpc1 rs1 m1 ss1)), lp)
-          ))
-        else if x64_decode xpc l_bin = Some(1,Pret) then
-          let (pc', ss', caller,fp) = update_stack2 ss in 
-          let rs' = restore_x64_caller rs caller fp in ((pc', Next xpc rs' m ss'), lp)
-          \<comment>\<open> case: NOT BPF JMP \<close>
-        else
-          ((pc+1, x64_sem num l_bin (Next xpc rs m ss)), lp)
-)))"
-*)
 lemma jitfix_induct:
   "jitfix (a#l_jump) l_bin0 l_pc = Some prog \<Longrightarrow> 
   \<exists> prog'. jitfix [a] l_bin0 l_pc = Some prog' \<and> jitfix l_jump prog' l_pc = Some prog"
@@ -139,24 +12,6 @@ lemma jitfix_induct:
 lemma jitfix_induct2:
   "\<exists> prog'. jitfix [a] l_bin0 l_pc = Some prog' \<and> jitfix l_jump prog' l_pc = Some prog \<Longrightarrow> jitfix (a#l_jump) l_bin0 l_pc = Some prog"
   by (metis (no_types, lifting) jitfix.elims jitfix.simps(1) jitfix.simps(2) option.case_eq_if option.discI option.inject)
-
-
-(*
-definition match_state2::"outcome \<Rightarrow> outcome \<Rightarrow> bool" where
-  "match_state2 fxst xxst \<equiv> 
-  (case fxst of (Next xst xrs xm xss) \<Rightarrow>
-    (case xxst of (Next xst1 xrs1 xm1 xss1) \<Rightarrow> 
-     xst = xst1 \<and> xrs = xrs1 \<and> xm = xm1 \<and> xss = xss1 |
-                   _ \<Rightarrow> False)|
-                 _ \<Rightarrow> False)"*)
-
-definition match_state2::"outcome \<Rightarrow> outcome \<Rightarrow> bool" where
-  "match_state2 fxst xxst \<equiv> 
-  fxst = xxst \<and> (fxst \<noteq> Stuck \<or> xxst \<noteq> Stuck)"
-
-
-definition jit_fix_sem::"nat \<Rightarrow> x64_bin \<Rightarrow> outcome \<Rightarrow> outcome" where
-  "jit_fix_sem n lt xst = x64_sem n lt xst"
 
 lemma jit_fix_not_change_length:
   "jitfix l_jump l_bin0 l_pc = Some prog \<Longrightarrow>
@@ -197,11 +52,38 @@ next
   then show ?case using Cons b0 b1 by argo
 qed
 
+lemma jit_fix_not_change:
+  "jitfix l_jump l_bin0 l_pc = Some prog \<Longrightarrow> 
+  x64_decode xpc l_bin0 = Some v \<Longrightarrow>
+  (\<not>(\<exists> num d. x64_decode xpc l_bin0 = Some(num, Pcall_i d))) \<and> (\<not> (\<exists> num cond d. x64_decode xpc l_bin0 = Some(num, Pjcc cond d))) \<Longrightarrow>
+  x64_decode xpc prog = Some v"
+  sorry
+
 (*\<and> x64_decode 0 l \<noteq> None \<and>*)
+(*
+lemma jit_fix_change:
+  "jitfix l_jump l_bin0 l_pc = Some prog \<Longrightarrow> 
+  x64_decode xpc l_bin0 = Some v \<Longrightarrow>
+  (\<exists> num d. x64_decode xpc l_bin0 = Some(num, Pcall_i d)) \<or> (\<exists> num src dst. x64_decode xpc l_bin0 = Some(num, Pjcc cond d)) \<Longrightarrow>
+  get_updated_l_bin x l l_pc 
+  x64_decode xpc prog = x"
+*)
+
+(*
 lemma jit_fix_not_change:
   "jitfix l_jump l_bin0 l_pc = Some prog \<Longrightarrow> 
   x64_decode xpc l_bin0 \<noteq> None \<Longrightarrow> 
-  (\<not>(\<exists> num. x64_decode xpc l_bin0 = Some(num,Pret))) \<and> (\<not>(\<exists> num d. x64_decode xpc l_bin0 = Some(num, Pcall_i d))) \<and> (\<not> (\<exists> num src dst. x64_decode xpc l_bin0 = Some(num, Pcmpq_rr src dst))) \<Longrightarrow>
+  (\<not>(\<exists> num d. x64_decode xpc l_bin0 = Some(num, Pcall_i d))) \<and> (\<not> (\<exists> num src dst. x64_decode xpc l_bin0 = Some(num, Pjcc cond d))) \<Longrightarrow>
+  list_in_list l xpc l_bin0 \<longrightarrow> list_in_list l xpc prog"
+  sorry
+*)
+
+
+(*
+lemma jit_fix_change:
+  "jitfix l_jump l_bin0 l_pc = Some prog \<Longrightarrow> 
+  x64_decode xpc l_bin0 \<noteq> None \<Longrightarrow> 
+  (\<exists> num d. x64_decode xpc l_bin0 = Some(num, Pcall_i d)) \<or> (\<exists> num src dst. x64_decode xpc l_bin0 = Some(num, Pjcc cond d)) \<Longrightarrow>
   list_in_list l xpc l_bin0 \<longrightarrow> list_in_list l xpc prog"
   sorry
 
@@ -215,8 +97,654 @@ lemma list_in_list_prop4: "
   fxst \<noteq> Stuck \<Longrightarrow>
   xxst = fxst"
   sorry
+*)
+
+lemma l_pc_index_corr2:
+  "find_target_pc_in_l_pc2 l_pc (int xpc) 0 = Some pc \<Longrightarrow> nat (fst (l_pc!(nat pc))) = xpc"
+  sorry
+
+
+(*lemma hh:
+  "prog = x64_bin_update (length u8_list) l_bin0 xpc u8_list \<Longrightarrow>
+  u8_list = x64_encode ins \<Longrightarrow>
+  x64_decode xpc l_bin0 = Some (len,ins) \<Longrightarrow>
+  x64_decode xpc prog = Some (len,ins)"
+  sorry*)
+
+lemma x64_bin_update_is_disjoint:
+  "jitfix [x] l_bin0 l_pc = Some prog' \<Longrightarrow>
+  jitfix l_jump l_bin0 l_pc = Some prog \<Longrightarrow>
+  x \<in> set l_jump \<Longrightarrow>
+  Some prog' = Some (x64_bin_update (length u8_list) l_bin0 xpc u8_list) \<Longrightarrow>
+  x64_decode xpc prog' = Some v \<Longrightarrow>
+  x64_decode xpc prog = Some v"
+  sorry
+
+
+
+lemma x64_bin_update_decode_incode_consistency:
+  "Some someprog = Some (x64_bin_update (length (x64_encode ins)) l_bin0 xpc (x64_encode ins)) \<Longrightarrow>
+  x64_decode xpc someprog = Some (length (x64_encode ins),ins)"
+  sorry
+
+lemma one_steps_equiv_layer3:
+  "fix_bpf_sem 1 (l_bin0,l_pc,l_jump) xst = fxst' \<Longrightarrow>
+  xst = Next xpc xrs xm xss \<Longrightarrow>
+  fxst' = Next xpc'' xrs'' xm'' xss'' \<Longrightarrow>
+  jitfix l_jump l_bin0 l_pc = Some prog \<Longrightarrow>  
+  jitflat_bpf lt init_second_layer = (l_bin0,l_pc,l_jump) \<Longrightarrow>
+  well_formed_prog lt \<Longrightarrow>
+  last_fix_sem 1 prog xst = fst' \<Longrightarrow>
+  match_state2 fst' fxst'"
+proof-
+  assume a0:"fix_bpf_sem 1 (l_bin0,l_pc,l_jump) xst = fxst'" and
+  a1:"fxst' = Next xpc'' xrs'' xm'' xss''" and
+  a2:"jitfix l_jump l_bin0 l_pc = Some prog" and
+  a3:"xst = Next xpc xrs xm xss" and
+  a4:"jitflat_bpf lt init_second_layer = (l_bin0,l_pc,l_jump)" and
+  a5:"well_formed_prog lt" and
+  a7:"last_fix_sem 1 prog xst = fst'"
+
+  have b0_1:"fxst' = fix_bpf_one_step (l_bin0,l_pc,l_jump) xst"
+    using a0 by simp
+  have c0_0:"fxst' = (case x64_decode xpc l_bin0 of 
+                  Some(sz, Pcall_i imm) \<Rightarrow>
+                      let v = find_target_pc_in_l_pc2 l_pc (int xpc) 0 in
+                      (case v of None \<Rightarrow> Stuck | Some pc \<Rightarrow>
+                      (case find_target_pc_in_l_pc l_jump pc of
+                        None \<Rightarrow> Stuck |
+                        Some npc \<Rightarrow>
+                      exec_instr (Pcall_i (of_int(fst (l_pc!(unat npc))))) sz xpc xrs xm xss)) |
+                  Some(sz, Pjcc cond d) \<Rightarrow> 
+                      let v = find_target_pc_in_l_pc2 l_pc (int xpc-3) 0 in
+                      (case v of None \<Rightarrow> Stuck | Some pc \<Rightarrow>
+                      (case find_target_pc_in_l_pc l_jump pc of
+                        None \<Rightarrow> Stuck |
+                        Some npc \<Rightarrow>
+                          (exec_instr (Pjcc cond (of_int (fst (l_pc!(unat npc)))-(of_nat (xpc+1)))) sz xpc xrs xm xss))) |
+                  Some(sz,ins) \<Rightarrow> (exec_instr ins sz xpc xrs xm xss) |
+                  _ \<Rightarrow> Stuck )"
+          using b0_1 a3 by(unfold fix_bpf_one_step_def Let_def,simp_all) 
+  thus ?thesis 
+  proof(cases "\<exists> num d. x64_decode xpc l_bin0 = Some(num, Pcall_i d)")
+    case True
+    then obtain sz d where b1:"x64_decode xpc l_bin0 = Some(sz, Pcall_i d)" by auto
+    have c0:"fxst' = (let v = find_target_pc_in_l_pc2 l_pc (int xpc) 0 in
+                      (case v of None \<Rightarrow> Stuck | Some pc \<Rightarrow>
+                      (case find_target_pc_in_l_pc l_jump pc of
+                        None \<Rightarrow> Stuck |
+                        Some npc \<Rightarrow>
+                      exec_instr (Pcall_i (of_int(fst (l_pc!(unat npc))))) sz xpc xrs xm xss)))" using b1 c0_0 by simp
+    
+    hence "find_target_pc_in_l_pc2 l_pc (int xpc) 0 \<noteq> None" using a1
+      using option.simps(4) by fastforce 
+    hence "\<exists> pc. find_target_pc_in_l_pc2 l_pc (int xpc) 0 = Some pc" by simp
+    then obtain pc where c1:"find_target_pc_in_l_pc2 l_pc (int xpc) 0 = Some pc" by auto
+    hence c2_0:"find_target_pc_in_l_pc l_jump pc \<noteq> None" using c0 a1
+      using option.simps(4) by fastforce 
+    hence "\<exists> npc. find_target_pc_in_l_pc l_jump pc = Some npc" by force 
+    then obtain npc where c2:"find_target_pc_in_l_pc l_jump pc = Some npc" by auto
+    have c3:"fxst' = exec_instr (Pcall_i (of_int(fst (l_pc!(unat npc))))) sz xpc xrs xm xss"
+      using c0 c1 c2 by simp
+
+    hence d0:"(pc,npc) \<in> set l_jump" using c1 c2 search_l_jump
+      by (metis a4 distinct.simps(1) init_second_layer_def is_increase_list_empty l_jump_is_distinct list.simps(8))
+    have "l_bin0 \<noteq> []"
+      by (metis c2_0 a2 find_target_pc_in_l_pc.simps(1) jitfix.elims option.simps(3)) 
+    hence "jitfix [(pc,npc)] l_bin0 l_pc = (let res = get_updated_l_bin (pc,npc) l_bin0 l_pc in case res of None \<Rightarrow> None | 
+                                                        Some l' \<Rightarrow> Some l')" by auto
+    hence d1:"jitfix [(pc,npc)] l_bin0 l_pc = get_updated_l_bin (pc,npc) l_bin0 l_pc" 
+      using a2 by(cases "get_updated_l_bin (pc,npc) l_bin0 l_pc",simp_all)
+    let "?prog" = "jitfix [(pc,npc)] l_bin0 l_pc"
+    have d2:"?prog = (let fix_begin_addr = fst (l_pc!(nat pc)); 
+        (target_begin_addr,num2) = l_pc!(unat npc) in 
+        (case x64_decode (nat fix_begin_addr) l_bin0 of 
+              Some(sz, Pcall_i _) \<Rightarrow> let u8_list = x64_encode (Pcall_i (of_int target_begin_addr)) in
+                                     Some (x64_bin_update (length u8_list) l_bin0 (nat fix_begin_addr) u8_list) |
+              Some(sz, Pcmpq_rr src dst) \<Rightarrow> let loc = nat fix_begin_addr+sz in 
+                    (case x64_decode loc l_bin0 of 
+                            Some(sz2, Pjcc cond _) \<Rightarrow> let offset = ((of_int target_begin_addr)::i32) - ((of_nat (loc+sz2)+1)::i32) in
+                                                      let u8_list = x64_encode (Pjcc cond (ucast offset)) in                                                     
+                                                      Some (x64_bin_update (length u8_list) l_bin0 loc u8_list) | 
+                            _ \<Rightarrow> None ) |
+              _ \<Rightarrow> None ))"
+      using get_updated_l_bin_def d1 by auto
+    have d2_0:"(fst (l_pc!(nat pc))) \<ge> 0" using a3 sorry
+    have d2_1:"nat (fst (l_pc!(nat pc))) = xpc" using l_pc_index_corr2 c1 by blast     
+    have d2_2:"(fst (l_pc!(nat pc))) = int xpc" using d2_1 d2_0 by presburger     
+    have d2_3:"of_int (int xpc) = of_nat xpc" using d2_0 by simp
+    let "?target_begin_addr" = "fst(l_pc!(unat npc))"
+    have "?prog = (
+        (case x64_decode xpc l_bin0 of 
+              Some(sz, Pcall_i _) \<Rightarrow> let u8_list = x64_encode (Pcall_i (of_int ?target_begin_addr)) in
+                                     Some (x64_bin_update (length u8_list) l_bin0 xpc u8_list) |
+              Some(sz, Pcmpq_rr src dst) \<Rightarrow> let loc = xpc+sz in 
+                    (case x64_decode loc l_bin0 of 
+                            Some(sz2, Pjcc cond _) \<Rightarrow> let offset = ((of_int ?target_begin_addr)::i32) - ((of_nat (loc+sz2)+1)::i32) in
+                                                      let u8_list = x64_encode (Pjcc cond (ucast offset)) in                                                     
+                                                      Some (x64_bin_update (length u8_list) l_bin0 loc u8_list) | 
+                            _ \<Rightarrow> None ) |
+              _ \<Rightarrow> None ))"
+      using d2_1 d2_2 d2_3 d2 sorry 
+    hence d3:"?prog = (let u8_list = x64_encode (Pcall_i (of_int ?target_begin_addr)) in
+                                     Some (x64_bin_update (length u8_list) l_bin0 xpc u8_list))"
+      using b1 by(cases "x64_decode xpc l_bin0",simp_all)
+    
+    let "?u8_list" = "(of_int ?target_begin_addr)"
+    let "?len_u8_list" = "length(x64_encode (Pcall_i (of_int ?target_begin_addr)))"
+    have "\<exists> someprog. ?prog = Some someprog" using a2 by (meson d3) 
+    then obtain someprog where d4:"?prog = Some someprog" by auto
+    hence d4_1:"Some someprog = Some (x64_bin_update (length (x64_encode (Pcall_i ?u8_list))) l_bin0 xpc (x64_encode (Pcall_i ?u8_list)))"
+      using d4 d3 by metis 
+    have "last_fix_sem 1 someprog xst = (x64_sem 1 someprog xst)" using last_fix_sem_def by blast
+    hence d5_1:"last_fix_sem 1 someprog xst = (case x64_decode xpc someprog of
+      None \<Rightarrow> Stuck |
+      Some (sz, ins) \<Rightarrow>
+       (exec_instr ins sz xpc xrs xm xss))" using a3
+      by (simp add: option.case_eq_if)  
+    have d5:"x64_decode xpc someprog = Some (?len_u8_list,Pcall_i ?u8_list)" 
+      using x64_bin_update_decode_incode_consistency d4_1 by blast
+    hence "?len_u8_list = sz" using b1 d5 sorry
+    (*exec_instr (Pcall_i (of_int(fst (l_pc!(unat npc))))) sz xpc xrs xm xss"*)
+    hence d5_2:"last_fix_sem 1 someprog xst = (exec_instr (Pcall_i ?u8_list) sz xpc xrs xm xss)"
+      using d5_1 d5 by simp
+    hence dn:"last_fix_sem 1 someprog xst = fxst'" using d5_2 c3 by metis
+
+    have e0:"last_fix_sem 1 prog xst = (case x64_decode xpc prog of
+      None \<Rightarrow> Stuck |
+      Some (sz, ins) \<Rightarrow>
+       (exec_instr ins sz xpc xrs xm xss))" using  a3 last_fix_sem_def by (simp add: option.case_eq_if)  
+
+    have e1:"x64_decode xpc someprog = x64_decode xpc prog" 
+      using x64_bin_update_is_disjoint a2 d0 d1 d3 d5 d4_1 by (smt (verit)) 
+    have e2:"last_fix_sem 1 prog xst = (exec_instr (Pcall_i ?u8_list) sz xpc xrs xm xss)"
+      using e0 e1 d5_1 d5_2 by argo 
+    
+    then show ?thesis using e2 dn match_state2_def a1 a7 d5_2 by fastforce 
+  next
+    case False
+    have b0:"\<not>(\<exists> num d. x64_decode xpc l_bin0 = Some(num, Pcall_i d))" using False by simp
+    then show ?thesis 
+    proof(cases "\<exists> num cond d. x64_decode xpc l_bin0 = Some(num, Pjcc cond d)")
+      case True 
+      then obtain sz cond d where b1:"x64_decode xpc l_bin0 = Some(sz, Pjcc cond d)" by auto
+      have c0:"fxst' = (let v = find_target_pc_in_l_pc2 l_pc (int xpc-3) 0 in
+                      (case v of None \<Rightarrow> Stuck | Some pc \<Rightarrow>
+                      (case find_target_pc_in_l_pc l_jump pc of
+                        None \<Rightarrow> Stuck |
+                        Some npc \<Rightarrow>
+                          (exec_instr (Pjcc cond (of_int (fst (l_pc!(unat npc)))-(of_nat (xpc+1)))) sz xpc xrs xm xss))))"
+        using c0_0 b1 by simp
+      have "\<exists> pc. find_target_pc_in_l_pc2 l_pc (int xpc-3) 0 = Some pc"
+        using c0 a1 option.simps(4) by fastforce 
+      then obtain pc where c1:"find_target_pc_in_l_pc2 l_pc (int xpc-3) 0 = Some pc" by auto
+      have "\<exists> npc. find_target_pc_in_l_pc l_jump pc = Some npc"
+        using c0 c1 a1 option.exhaust_sel by fastforce
+      then obtain npc where c2:"find_target_pc_in_l_pc l_jump pc = Some npc" by auto
+      have c3:"fxst' = (exec_instr (Pjcc cond (of_int (fst (l_pc!(unat npc)))-(of_nat (xpc+1)))) sz xpc xrs xm xss)"
+        using c0 c2 c1 by force
+
+      have d0:"(pc,npc) \<in> set l_jump" using c2 search_l_jump
+        by (metis a4 distinct.simps(1) init_second_layer_def is_increase_list_empty l_jump_is_distinct list.simps(8)) 
+      have "l_bin0 \<noteq> []" using a2
+        by (metis c2 find_target_pc_in_l_pc.simps(1) jitfix.simps(2) list.exhaust option.distinct(1)) 
+       hence "jitfix [(pc,npc)] l_bin0 l_pc = (let res = get_updated_l_bin (pc,npc) l_bin0 l_pc in case res of None \<Rightarrow> None | 
+                                                        Some l' \<Rightarrow> Some l')" by auto
+    hence d1:"jitfix [(pc,npc)] l_bin0 l_pc = get_updated_l_bin (pc,npc) l_bin0 l_pc" 
+      using a2 by(cases "get_updated_l_bin (pc,npc) l_bin0 l_pc",simp_all)
+    let "?prog" = "jitfix [(pc,npc)] l_bin0 l_pc"
+    have d2:"?prog = (let fix_begin_addr = fst (l_pc!(nat pc)); 
+        (target_begin_addr,num2) = l_pc!(unat npc) in 
+        (case x64_decode (nat fix_begin_addr) l_bin0 of 
+              Some(sz, Pcall_i _) \<Rightarrow> let u8_list = x64_encode (Pcall_i (of_int target_begin_addr)) in
+                                     Some (x64_bin_update (length u8_list) l_bin0 (nat fix_begin_addr) u8_list) |
+              Some(sz, Pcmpq_rr src dst) \<Rightarrow> let loc = nat fix_begin_addr+sz in 
+                    (case x64_decode loc l_bin0 of 
+                            Some(sz2, Pjcc cond _) \<Rightarrow> let offset = ((of_int target_begin_addr)::i32) - ((of_nat (loc+sz2)+1)::i32) in
+                                                      let u8_list = x64_encode (Pjcc cond (ucast offset)) in                                                     
+                                                      Some (x64_bin_update (length u8_list) l_bin0 loc u8_list) | 
+                            _ \<Rightarrow> None ) |
+              _ \<Rightarrow> None ))"
+      using get_updated_l_bin_def d1 by auto
+    have d2_0:"(fst (l_pc!(nat pc))) \<ge> 0" using a3 sorry
+    have d2_1:"nat (fst (l_pc!(nat pc))) = xpc" using l_pc_index_corr2 c1 sorry
+    have d2_2:"(fst (l_pc!(nat pc))) = int xpc" using d2_1 d2_0 by presburger     
+    have d2_3:"of_int (int xpc) = of_nat xpc" using d2_0 by simp
+    let "?target_begin_addr" = "fst(l_pc!(unat npc))"
+    have "?prog = (
+        (case x64_decode xpc l_bin0 of 
+              Some(sz, Pcall_i _) \<Rightarrow> let u8_list = x64_encode (Pcall_i (of_int ?target_begin_addr)) in
+                                     Some (x64_bin_update (length u8_list) l_bin0 xpc u8_list) |
+              Some(sz, Pcmpq_rr src dst) \<Rightarrow> let loc = xpc+sz in 
+                    (case x64_decode loc l_bin0 of 
+                            Some(sz2, Pjcc cond _) \<Rightarrow> let offset = ((of_int ?target_begin_addr)::i32) - ((of_nat (loc+sz2)+1)::i32) in
+                                                      let u8_list = x64_encode (Pjcc cond (ucast offset)) in                                                     
+                                                      Some (x64_bin_update (length u8_list) l_bin0 loc u8_list) | 
+                            _ \<Rightarrow> None ) |
+              _ \<Rightarrow> None ))"
+      using d2_1 d2_2 d2_3 d2 sorry 
+      thus ?thesis sorry
+      (*have c0_0:"\<exists> num src dst. x64_decode xpc l_bin0 = Some(num, Pjcc cond d)" using True by simp
+      then obtain num src dst where c0_1:"x64_decode xpc l_bin0 = Some(num, Pcmpq_rr src dst)" by auto
+      have c0:"snd fxst' = snd (let num = snd (l_pc!(unat pc)) in case x64_sem num l_bin0 (Next xpc xrs xm xss) of
+          Stuck \<Rightarrow> (pc, Stuck) | \<comment>\<open> if one step error, stop, it should be impossible \<close>
+          Next xpc1 rs1 m1 ss1 \<Rightarrow> (
+            if rs1 (CR ZF) = 1 then \<comment>\<open> must JUMP \<close>
+              (case find_target_pc_in_l_pc l_jump (uint pc) of
+              None \<Rightarrow> (pc, Stuck) |
+              Some npc \<Rightarrow>
+                (npc, (Next (nat (fst (l_pc!(unat npc)))) rs1 m1 ss1))) \<comment>\<open> go to the target address in the jited x64 binary \<close>
+            else \<comment>\<open> donot JUMP \<close>
+              (pc+1, (Next xpc1 rs1 m1 ss1))
+          ))" using True a0 b0_1 a3 a6 b0_3 a1
+        apply(unfold flat_bpf_one_step_def Let_def,simp_all) 
+        apply(cases "x64_decode xpc l_bin0",simp_all)
+        subgoal for a apply(split if_splits,simp_all)
+          done
+        done
+      let "?num" = "(snd (l_pc!(unat pc)))"
+      have "\<exists> fxst1. fxst1 = x64_sem ?num l_bin0 (Next xpc xrs xm xss)" by fastforce
+      then obtain fxst1 where c1:"fxst1 = x64_sem ?num l_bin0 (Next xpc xrs xm xss)" by auto
+      have "fxst1 \<noteq> Stuck" using c0 a1 c1 by(cases "x64_sem ?num l_bin0 (Next xpc xrs xm xss)",simp_all)
+      hence "\<exists> xpc1 xrs1 xm1 xss1. Next xpc1 xrs1 xm1 xss1 = fxst1"
+        by (metis outcome.exhaust) 
+      then obtain xpc1 xrs1 xm1 xss1 where c2:"Next xpc1 xrs1 xm1 xss1 = fxst1" by auto
+      have c3_0:"snd fxst' = snd (if xrs1 (CR ZF) = 1 then \<comment>\<open> must JUMP \<close>
+              (case find_target_pc_in_l_pc l_jump (uint pc) of
+              None \<Rightarrow> (pc, Stuck) |
+              Some npc \<Rightarrow>
+                (npc, (Next (nat (fst (l_pc!(unat npc)))) xrs1 xm1 xss1))) \<comment>\<open> go to the target address in the jited x64 binary \<close>
+            else \<comment>\<open> donot JUMP \<close>
+              (pc+1, (Next xpc1 xrs1 xm1 xss1))
+          )" using c2 c1 c0
+        by (metis (no_types, lifting) outcome.simps(4)) 
+      thus ?thesis
+      proof(cases "xrs1 (CR ZF) = 1")
+        case True
+        have b1:"xrs1 (CR ZF) = 1" using True by simp
+        then show ?thesis
+            proof(cases "find_target_pc_in_l_pc l_jump (uint pc) \<noteq> None")
+              case True
+                have "\<exists> npc. find_target_pc_in_l_pc l_jump (uint pc) = Some npc" using True by simp
+                then obtain npc where c3_1:"find_target_pc_in_l_pc l_jump (uint pc) = Some npc" by auto                                 
+                have c3:"snd fxst' = (Next (nat (fst (l_pc!(unat npc)))) xrs1 xm1 xss1)" 
+                  using True c3_0 c3_1 b1 by simp
+                have "distinct (map fst l_jump)" using init_second_layer_def a4 is_increase_list_empty
+                  by (metis distinct.simps(1) l_jump_is_distinct list.simps(8)) 
+                hence d0:"(uint pc,npc) \<in> set l_jump" using c3_1 search_l_jump by auto
+                have d1_1:"l_bin0 \<noteq> []" using a2
+                  by (metis True find_target_pc_in_l_pc.simps(1) jitfix.elims option.distinct(1)) 
+                hence "jitfix [(uint pc,npc)] l_bin0 l_pc = get_updated_l_bin (uint pc,npc) l_bin0 l_pc" 
+                  by(cases "get_updated_l_bin (uint pc,npc) l_bin0 l_pc",simp_all)
+                hence d1:"jitfix [(uint pc,npc)] l_bin0 l_pc = (let fix_begin_addr = fst (l_pc!(nat(uint pc))); 
+        (target_begin_addr,num2) = l_pc!(unat npc) in 
+        (case x64_decode (nat fix_begin_addr) l_bin0 of 
+              Some(sz, Pcall_i _) \<Rightarrow> let offset = ((of_int target_begin_addr)::i32) - ((of_int fix_begin_addr+of_nat sz+1)::i32) in 
+                                     let u8_list = x64_encode (Pcall_i (ucast offset)) in
+                                     Some (x64_bin_update (length u8_list) l_bin0 (nat fix_begin_addr) u8_list) |
+              Some(sz, Pcmpq_rr src dst) \<Rightarrow> let loc = nat fix_begin_addr+sz in 
+                    (case x64_decode loc l_bin0 of 
+                            Some(sz2, Pjcc cond _) \<Rightarrow> let offset = ((of_int target_begin_addr)::i32) - ((of_nat (loc+sz2)+1)::i32) in
+                                                      let u8_list = x64_encode (Pjcc cond (ucast offset)) in                                                     
+                                                      Some (x64_bin_update (length u8_list) l_bin0 loc u8_list) | 
+                            _ \<Rightarrow> None ) |
+              _ \<Rightarrow> None ))" using get_updated_l_bin_def by simp
+
+                let "?fix_begin_addr" = "fst (l_pc!(nat(uint pc)))"
+                let "?target_begin_addr" = "fst (l_pc!(unat npc))"
+                have d2:"nat ?fix_begin_addr = xpc" using b0_2 by auto
+                hence "\<exists> sz src dst. x64_decode (nat ?fix_begin_addr) l_bin0 = Some(sz, Pcmpq_rr src dst)" using c0_0 by force 
+                then obtain sz src dst where d3_1:"x64_decode (nat ?fix_begin_addr) l_bin0 = Some(sz, Pcmpq_rr src dst)" by auto
+                hence d3:"jitfix [(uint pc,npc)] l_bin0 l_pc =  (let loc = nat ?fix_begin_addr+sz in 
+                    (case x64_decode loc l_bin0 of 
+                            Some(sz2, Pjcc cond _) \<Rightarrow> let offset = ((of_int ?target_begin_addr)::i32) - ((of_nat (loc+sz2)+1)::i32) in
+                                                      let u8_list = x64_encode (Pjcc cond (ucast offset)) in                                                     
+                                                      Some (x64_bin_update (length u8_list) l_bin0 loc u8_list) | 
+                            _ \<Rightarrow> None ))" using d1 d2 d1_1
+                  apply(cases "x64_decode (nat ?fix_begin_addr) l_bin0",simp_all)
+                  subgoal for a apply(cases "l_pc ! unat npc",simp_all)
+                    subgoal for aa b
+                    proof -
+                      assume "nat (fst (l_pc ! unat pc)) = xpc"
+                      assume "(case get_updated_l_bin (uint pc, npc) l_bin0 l_pc of None \<Rightarrow> None | Some x \<Rightarrow> Some x) = 
+                          (let loc = xpc + sz in case x64_decode loc l_bin0 of None \<Rightarrow> None | Some (sz2, Pjcc cond x) \<Rightarrow> 
+                           let offset = word_of_int aa - (word_of_nat (loc + sz2) + (1::32 signed word)); 
+                               u8_list = x64_encode (Pjcc cond (ucast offset)) in Some (x64_bin_update (length u8_list) l_bin0 loc u8_list) | Some (sz2, _) \<Rightarrow> None)"
+                      assume a1: "l_pc ! unat npc = (aa, b)"
+                      have "\<forall>i n. fst (i::int, n::nat) = i"
+                        by simp
+                      then show ?thesis
+                        using a1 by presburger
+                    qed 
+                    done
+                  done
+                have "jitfix [(uint pc,npc)] l_bin0 l_pc \<noteq> None"
+                proof(rule ccontr)
+                  assume assm:"\<not> (jitfix [(uint pc,npc)] l_bin0 l_pc\<noteq> None)"
+                  have "jitfix [(uint pc,npc)] l_bin0 l_pc = None" using assm by simp
+                  hence "jitfix l_jump l_bin0 l_pc = None " using d0 sorry
+                  thus "False" using a2 by simp
+                qed
+                hence "\<exists> prog'. Some prog' = jitfix [(uint pc,npc)] l_bin0 l_pc"
+                  by force
+                then obtain prog' where "Some prog' = jitfix [(uint pc,npc)] l_bin0 l_pc" by auto
+                hence "prog' = (let loc = nat ?fix_begin_addr+sz in 
+                    (case x64_decode loc l_bin0 of 
+                            Some(sz2, Pjcc cond _) \<Rightarrow> let offset = ((of_int ?target_begin_addr)::i32) - ((of_nat (loc+sz2)+1)::i32) in
+                                                      let u8_list = x64_encode (Pjcc cond (ucast offset)) in                                                     
+                                                      (x64_bin_update (length u8_list) l_bin0 loc u8_list)))"
+                  using d3 apply(cases "x64_decode (nat ?fix_begin_addr+sz) l_bin0",simp_all)
+                  subgoal for a apply(cases a,simp_all)
+                    subgoal for aa b apply(cases b,simp_all)
+                      subgoal for x131 x132
+                        by (meson option.inject)
+                      done
+                    done
+                  done
+                
+                have "last_fix_sem 2 prog' xst = x64_sem 2 prog' xst" using last_fix_sem_def by simp
+                hence e0_0:"last_fix_sem 2 prog' xst =  (
+                  case x64_decode xpc prog' of
+                  None \<Rightarrow> Stuck |
+                  Some (sz, ins) \<Rightarrow>
+                    x64_sem 1 prog' (exec_instr ins sz xpc xrs xm xss)
+                )"  by (metis Suc_1 a3 x64_sem.simps(3)) 
+
+               (* have "list_in_list (x64_encode(Pcmpq_rr src dst)) xpc l_bin0" using d2 d3_1 
+                proof(rule ccontr)
+                  assume assm:"\<not> (list_in_list (x64_encode(Pcmpq_rr src dst)) xpc l_bin0)"
+                  have "\<not> (x64_decode xpc l_bin0 = Some (length (x64_encode(Pcmpq_rr src dst)), Pcmpq_rr src dst))" using x64_encode_decode_consistency assm 
+                  have e0:"x64_decode xpc prog' = x64_decode xpc l_bin0" 
+                  proof(rule ccontr)*)
+
+                hence e1:"last_fix_sem 2 prog' xst =  (
+                  case x64_decode xpc prog' of
+                  Some (sz, Pcmpq_rr src dst) \<Rightarrow>
+                    x64_sem 1 prog' (exec_instr (Pcmpq_rr src dst) sz xpc xrs xm xss)
+                )" using c0_0 a3 e0_0 apply(cases "x64_decode xpc prog'",simp_all) sorry
+                
+                have "last_fix_sem 2 prog xst = x64_sem 2 prog xst" using last_fix_sem_def by simp
+                hence e0:"last_fix_sem 2 prog xst =  (
+                  case x64_decode xpc prog of
+                  None \<Rightarrow> Stuck |
+                  Some (sz, ins) \<Rightarrow>
+                    x64_sem 1 prog (exec_instr ins sz xpc xrs xm xss)
+                )"
+                  by (metis Suc_1 a3 x64_sem.simps(3)) 
+                have e1:"\<exists> num src dst. x64_decode xpc prog = Some(num, Pcmpq_rr src dst)" sorry
+                hence "\<exists> src dst sz. last_fix_sem 2 prog xst = x64_sem 1 prog (exec_instr (Pcmpq_rr src dst) sz xpc xrs xm xss)"
+                  using e0 e1 by force
+                then obtain src dst sz where e2:"last_fix_sem 2 prog xst = x64_sem 1 prog (exec_instr (Pcmpq_rr src dst) sz xpc xrs xm xss)" by auto
+                hence e3:"sz = 3" using x64_encode_decode_consistency x64_encode_def list_in_list_prop sorry
+
+              then show ?thesis sorry
+            next
+              case False
+              then show ?thesis sorry
+            qed
+      next
+        case False
+        then show ?thesis sorry
+      qed*)
+    next
+      case False
+       have b0_0:"(\<not>(\<exists> num d. x64_decode xpc l_bin0 = Some(num, Pcall_i d))) \<and> (\<not> (\<exists> num cond d. x64_decode xpc l_bin0 = Some(num, Pjcc cond d)))"
+          using False b0 by blast
+        
+       have b0_2:"x64_decode xpc l_bin0 \<noteq> None" 
+        proof(rule ccontr)
+          assume assm:"\<not> (x64_decode xpc l_bin0 \<noteq> None)"
+          have "x64_decode xpc l_bin0 = None" using assm by blast   
+          hence c0:"fxst' = Stuck" 
+            using b0_0 b0_1 fix_bpf_one_step_def a3 by(cases "x64_decode xpc l_bin0",simp_all) 
+          thus "False" using a1 by auto
+        qed
+
+        hence "\<exists> sz ins. x64_decode xpc l_bin0 = Some(sz,ins)" by auto
+        then obtain sz ins where b2:"x64_decode xpc l_bin0 = Some(sz,ins)" by auto
+        hence c1:"fxst' = exec_instr ins sz xpc xrs xm xss" 
+          using b2 b0_0 c0_0 apply(cases "x64_decode xpc l_bin0",simp_all) by(cases ins,simp_all)
+        have d0:"x64_decode xpc prog = Some(sz,ins)"
+          using jit_fix_not_change b2 a2 b0_0 by blast
+        hence d1:"fst' = (exec_instr ins sz xpc xrs xm xss)"
+          using a3 a7 apply(unfold last_fix_sem_def) by(cases "x64_decode xpc prog",simp_all)
+        thus ?thesis using c1 d1 match_state2_def a1 by fastforce
+        qed
+      qed
+    qed
+
+(*
+(*(l_bin0,l_pc,l_jump) *)
+lemma n_steps_equiv_layer2:
+  "flat_bpf_sem n (l_bin0,l_pc,l_jump) (pc,xst) = fxst' \<Longrightarrow>
+  xst = Next xpc xrs xm xss \<Longrightarrow>
+  snd fxst' = Next xpc'' xrs'' xm'' xss'' \<Longrightarrow>
+  jitfix l_jump l_bin0 l_pc = Some prog \<Longrightarrow>
+  jitflat_bpf lt init_second_layer = (l_bin0,l_pc,l_jump) \<Longrightarrow>
+  well_formed_prog lt \<Longrightarrow>
+  \<exists> num fst'. last_fix_sem num prog xst = fst' \<and> match_state2 fst' (snd fxst')"
+proof(induct n arbitrary:l_bin0 l_pc l_jump pc xst fxst' xpc xrs xm xss xpc'' xrs'' xm'' xss'' prog lt)
+  case 0 
+  assume assm0:"flat_bpf_sem 0 (l_bin0,l_pc,l_jump) (pc,xst) = fxst'" and
+    assm1:"xst = Next xpc xrs xm xss" and
+    assm2:"snd fxst' = Next xpc'' xrs'' xm'' xss''" and
+    assm3:"jitfix l_jump l_bin0 l_pc = Some prog" and
+    assm4:"jitflat_bpf lt init_second_layer = (l_bin0,l_pc,l_jump)" and
+    assm5:"well_formed_prog lt" 
+  have a0:"last_fix_sem 0 prog xst = xst"  by (simp add: last_fix_sem_def) 
+  have a1:"snd (flat_bpf_sem 0 (l_bin0,l_pc,l_jump) (pc,xst)) = xst" by simp
+
+  have "\<exists> num fst'. num = 0 \<and> last_fix_sem num prog xst = fst'" using a0 by blast
+
+  hence "\<exists> num fst'. num = 0 \<and> last_fix_sem num prog xst = fst' \<and> match_state2 fst' (snd fxst')"
+  using a0 a1 apply(unfold match_state2_def last_fix_sem_def,simp_all) 
+    using assm1 assm0 apply(cases fxst') 
+    subgoal for a b apply(cases fxst')
+      subgoal for aa ba apply(cases xst)
+        subgoal for x11 x12 x13 x14 apply(cases xst,simp_all)
+          subgoal for x11a by(cases b,simp_all)
+          done
+        apply(cases xst,simp_all)
+          done
+        done
+      done
+           
+  then show ?case by blast
+    (*by (smt (verit, ccfv_threshold) flat_bpf_sem.simps(1) last_fix_sem_def match_state2_def outcome.simps(4) snd_conv x64_sem.simps(1))*) 
+next
+  case (Suc n)
+  assume assm0:"flat_bpf_sem (Suc n) (l_bin0,l_pc,l_jump) (pc,xst) = fxst'" and
+    assm1:"xst = Next xpc xrs xm xss" and
+    assm2:"snd fxst' = Next xpc'' xrs'' xm'' xss''" and
+    assm3:"jitfix l_jump l_bin0 l_pc = Some prog"
+  have "\<exists> next_f. flat_bpf_sem 1 (l_bin0,l_pc,l_jump) (pc,xst) = next_f" by blast
+  then obtain next_f where b0:"flat_bpf_sem 1 (l_bin0,l_pc,l_jump) (pc,xst) = next_f" by auto
+  have "unat pc < length lt \<and> unat pc \<ge> 0" 
+  proof(rule ccontr)
+    assume assm:"\<not> (unat pc < length lt \<and> unat pc \<ge> 0)"
+    have "snd next_f = snd (let pair = flat_bpf_one_step (l_bin0,l_pc,l_jump) (pc, xst) in
+    flat_bpf_sem 0 (l_bin0,l_pc,l_jump) pair)" 
+      using b0 by fastforce
+    hence "snd next_f = snd (flat_bpf_one_step (l_bin0,l_pc,l_jump) (pc, xst))"
+      by (metis flat_bpf_sem.simps(1) prod.collapse) 
+    hence "snd next_f = Stuck" 
+      using flat_bpf_one_step_def assm assm2 apply(cases xst,simp_all)
+      subgoal for x11 x12 x13 x14 apply(cases "(l_bin0,l_pc,l_jump)",simp_all)
+        subgoal for a 
+          by (smt (z3) Suc.prems(5) add.right_neutral init_second_layer_def l_pc_length_prop list.size(3) nat_le_linear nat_less_le)
+        done
+      done
+      thus "False" using assm2
+        by (metis assm0 b0 err_is_still_err3 flat_bpf_sem_induct_aux2 outcome.distinct(1) prod.collapse) 
+  qed
+
+  hence "\<exists> num next_s. last_fix_sem num prog xst = next_s \<and> match_state2 next_s (snd next_f)"
+    using one_steps_equiv_layer2 b0 assm0 assm2 assm3 flat_bpf_sem_induct_aux2 intermediate_step_is_ok3
+    by (metis (no_types, lifting) One_nat_def Suc.prems(2) Suc.prems(5) Suc.prems(6) less_eq_nat.simps(1) old.prod.exhaust snd_conv)  
+  then obtain num next_s where b1:"last_fix_sem num prog xst = next_s \<and> match_state2 next_s (snd next_f)" by auto
+  have "\<exists> xpc' xrs' xm' xss'. snd next_f = Next xpc' xrs' xm' xss'"
+    by (metis Suc.prems(3) assm0 b0 flat_bpf_sem_induct_aux2 intermediate_step_is_ok3 less_eq_nat.simps(1) outcome.distinct(1) prod.collapse)
+  then obtain xpc' xrs' xm' xss' where b2:"snd next_f = Next xpc' xrs' xm' xss'" by auto
+  have b3:"flat_bpf_sem n (l_bin0,l_pc,l_jump) next_f = fxst'" using flat_bpf_sem_induct_aux2 b0 assm0 by blast 
+  have "flat_bpf_sem n (l_bin0, l_pc, l_jump) (pc, xst) = fxst' \<Longrightarrow>
+      xst = Next xpc xrs xm xss \<Longrightarrow> 
+      snd fxst' = Next xpc'' xrs'' xm'' xss'' \<Longrightarrow> 
+      jitfix l_jump l_bin0 l_pc = Some prog \<Longrightarrow> 
+      \<exists>(num::nat) fst'::outcome. last_fix_sem num prog xst = fst' \<and> match_state2 fst' (snd fxst')" using Suc by simp
+  hence "\<exists>(num::nat) fst'::outcome. last_fix_sem num prog (snd next_f) = fst' \<and> match_state2 fst' (snd fxst')" 
+    using b2 b1 match_state2_def assm3 b0 assm2 b3
+    by (metis Suc.hyps Suc.prems(5) Suc.prems(6) prod.collapse) 
+    
+  then show ?case
+    by (metis Suc.prems(2) b1 last_fix_sem_def match_state2_def x64_sem_add) 
+qed
+
+
+lemma n_steps_equiv:
+  assumes assm0:"perir_sem n lt (pc,xxst) = xxst'" and
+  assm1:"xxst = Next xpc xrs xm xss" and
+  assm2:"snd xxst' = Next xpc' xrs' xm' xss'" and
+  assm3:"JITFlattern_def.match_state (pc,xxst) (pc,fxst)" and
+  assm4:"lt \<noteq> []" and
+  assm5:"well_formed_prog lt"and
+
+  assm6:"jitflat_bpf lt init_second_layer = (l_bin0,l_pc,l_jump)" and
+  assm7:"flat_bpf_sem n (l_bin0,l_pc,l_jump) (pc,fxst) = fxst'" and
+  assm8:"snd fxst' = Next xpc'' xrs'' xm'' xss''" and
+
+  assm9:"jitfix l_jump l_bin0 l_pc = Some prog" and
+  (*assm10:"last_fix_sem n prog xst = fst'" and*)
+  assm11:"jitper insns = Some lt"
+  shows "\<exists> num fst'. last_fix_sem num prog fxst = fst' \<and> match_state1 fst' (snd xxst')"
+proof-
+  have b0:"JITFlattern_def.match_state xxst' fxst'" 
+    using n_steps_equiv_layer1 assm3 assm0 assm1 assm2 assm4 assm5 assm11 assm6 assm7 assm8 by auto 
+  have "\<exists> xpc1 xrs xm xss. fxst = Next xpc1 xrs xm xss" 
+    using JITFlattern_def.match_state_def assm1 assm3 
+    apply(cases xxst,simp_all) 
+    apply(cases fxst,simp_all)
+    done
+  then obtain xpc1 xrs xm xss where b1:"fxst = Next xpc1 xrs xm xss" by auto
+  have b2:"\<exists> num fst'. last_fix_sem num prog fxst = fst' \<and> match_state2 fst' (snd fxst')" 
+    using n_steps_equiv_layer2 assm7 assm9 b1 assm8 assm6 assm5 by blast
+  then obtain num fst' where b3:"last_fix_sem num prog fxst = fst' \<and> match_state2 fst' (snd fxst')" by auto
+  hence b4:"match_state1 fst' (snd xxst')"
+    apply(unfold JITFlattern_def.match_state_def match_state2_def,simp_all)
+    using assm2 assm8 b0 b3
+    apply(cases fst',simp_all)
+    apply(cases "snd fxst'",simp_all)
+    apply(cases "snd xxst'",simp_all) 
+    subgoal for x11 x11a 
+      apply(cases "snd fxst'",simp_all)
+      subgoal for x11b
+        apply(unfold JITFlattern_def.match_state_def match_state2_def match_state1_def,simp_all)
+        apply(cases xxst',simp_all)
+        subgoal for a b 
+          apply(cases fxst',simp_all)
+          done
+        done
+      done
+    done
+  have "\<exists> num fst'. last_fix_sem num prog fxst = fst' \<and> match_state1 fst' (snd xxst')" using b2 b4 b3 by blast
+  thus ?thesis using b2 by auto
+qed
+*)
+
+lemma n_steps_equiv_layer3:
+  "fix_bpf_sem n (l_bin0,l_pc,l_jump) xst = fxst' \<Longrightarrow>
+  xst = Next xpc xrs xm xss \<Longrightarrow>
+  fxst' = Next xpc'' xrs'' xm'' xss'' \<Longrightarrow>
+  jitfix l_jump l_bin0 l_pc = Some prog \<Longrightarrow>  
+  jitflat_bpf lt init_second_layer = (l_bin0,l_pc,l_jump) \<Longrightarrow>
+  well_formed_prog lt \<Longrightarrow>
+  last_fix_sem n prog xst = fst' \<Longrightarrow>
+  match_state2 fst' fxst'"
+proof(induct n arbitrary:l_bin0 l_pc l_jump xst fxst' xpc xrs xm xss xpc'' xrs'' xm'' xss'' prog lt fst')
+  case 0 
+  then show ?case using last_fix_sem_def match_state2_def by auto 
+    (*by (smt (verit, ccfv_threshold) flat_bpf_sem.simps(1) last_fix_sem_def match_state2_def outcome.simps(4) snd_conv x64_sem.simps(1))*) 
+next
+  case (Suc n)
+  assume assm0:"fix_bpf_sem (Suc n) (l_bin0,l_pc,l_jump) xst = fxst'" and
+    assm1:"xst = Next xpc xrs xm xss" and
+    assm2:"fxst' = Next xpc'' xrs'' xm'' xss''" and
+    assm3:"jitfix l_jump l_bin0 l_pc = Some prog" and
+    assm4:"jitflat_bpf lt init_second_layer = (l_bin0,l_pc,l_jump)" and
+    assm5:"well_formed_prog lt" and
+    assm6:"last_fix_sem (Suc n) prog xst = fst'"
+ 
+  have "\<exists> next_f. fix_bpf_sem 1 (l_bin0,l_pc,l_jump) xst = next_f" by blast
+  then obtain next_f where b0:"fix_bpf_sem 1 (l_bin0,l_pc,l_jump) xst = next_f" by auto
+  have "\<exists> xpc' xrs' xm' xss'. next_f = Next xpc' xrs' xm' xss'"
+    using assm0 assm2 b0 by (metis One_nat_def err_is_still_err4 fix_bpf_sem.simps(1) fix_bpf_sem.simps(2) outcome.exhaust)
+  then obtain xpc' xrs' xm' xss' where b2:"next_f = Next xpc' xrs' xm' xss'" by auto
+
+  have "\<exists> next_s. last_fix_sem 1 prog xst = next_s" by blast
+  then obtain next_s where b1:"last_fix_sem 1 prog xst = next_s" by auto
+  hence bn:"match_state2 next_s next_f"
+    using one_steps_equiv_layer3 assm0 assm2 assm3 assm5 b0 b1 b2 match_state2_def assm1 assm4 by blast 
+ 
+  have b3:"fix_bpf_sem n (l_bin0,l_pc,l_jump) next_f = fxst'" using assm0 b0 by auto
+    
+  have b4:"last_fix_sem n prog next_s = fst'" using b1 assm6 last_fix_sem_def
+    by (metis Suc.prems(2) plus_1_eq_Suc x64_sem_add) 
+
+  then show ?case using match_state2_def b3 b4 b2
+    by (metis Suc.hyps Suc.prems(3) assm3 assm4 assm5 bn) 
+qed
+
+
+lemma n_steps_equiv:
+  assumes assm0:"perir_sem n lt (pc,xxst) = xxst'" and
+  assm1:"xxst = Next xpc xrs xm xss" and
+  assm2:"snd xxst' = Next xpc' xrs' xm' xss'" and
+  assm3:"JITFlattern_def.match_state (pc,fxst) (pc,xxst)" and
+  assm4:"lt \<noteq> []" and
+  assm5:"well_formed_prog lt"and
+
+  assm6:"jitflat_bpf lt init_second_layer = (l_bin0,l_pc,l_jump)" and
+  assm7:"flat_bpf_sem n (l_bin0,l_pc,l_jump) (pc,fxst) = fxst'" and
+  assm8:"snd fxst' = Next xpc'' xrs'' xm'' xss''" and
+
+  assm9:"jitfix l_jump l_bin0 l_pc = Some prog" and
+  assm10:"jitper insns = Some lt" and
+  assm11:"jitper insns = Some lt"
+  shows "\<exists> num fst'. last_fix_sem num prog fxst = fst' \<and> match_state1 fst' (snd xxst')" 
+proof-
+  have b0:"JITFlattern_def.match_state fxst' xxst'" 
+    using n_steps_equiv_layer1 assm3 assm0 assm1 assm2 assm4 assm5 assm11 assm6 assm7 assm8 match_mem_def assm10 by simp
+  have "\<exists> xpc1 xrs xm xss. fxst = Next xpc1 xrs xm xss" 
+    using JITFlattern_def.match_state_def assm1 assm3 
+    apply(cases xxst,simp_all) 
+    apply(cases fxst,simp_all)
+    done
+  then obtain xpc1 xrs xm xss where b1:"fxst = Next xpc1 xrs xm xss" by auto
+  have b2:"\<exists> num fst'. last_fix_sem num prog fxst = fst' \<and> match_state2 fst' (snd fxst')" 
+    using n_steps_equiv_layer2 assm7 assm9 b1 assm8 assm6 assm5 by (metis assm11 match_state2_def n_steps_equiv_layer3)
+  then obtain num fst' where b3:"last_fix_sem num prog fxst = fst' \<and> match_state2 fst' (snd fxst')" by auto
+  hence b4:"match_state1 fst' (snd xxst')"
+    apply(unfold JITFlattern_def.match_state_def match_state2_def,simp_all)
+    using assm2 assm8 b0 b3
+    apply(cases fst',simp_all)
+    apply(cases "snd fxst'",simp_all)
+    apply(cases "snd xxst'",simp_all) 
+    subgoal for x11 x11a 
+      apply(cases "snd fxst'",simp_all)
+      subgoal for x11b
+        apply(unfold JITFlattern_def.match_state_def match_state2_def match_state1_def,simp_all)
+        apply(cases xxst',simp_all)
+        subgoal for a b 
+          apply(cases fxst',simp_all)
+          done
+        done
+      done
+    done
+  have "\<exists> num fst'. last_fix_sem num prog fxst = fst' \<and> match_state1 fst' (snd xxst')" using b2 b4 b3 by blast
+  thus ?thesis using b2 by auto
+qed
 
 (*num = snd (l_pc!(unat pc))*)
+(*
 lemma one_steps_equiv_layer2:
   "flat_bpf_sem 1 (l_bin0,l_pc,l_jump) (pc,xst) = fxst' \<Longrightarrow>
   xst = Next xpc xrs xm xss \<Longrightarrow>
@@ -225,7 +753,7 @@ lemma one_steps_equiv_layer2:
   jitflat_bpf lt init_second_layer = (l_bin0,l_pc,l_jump) \<Longrightarrow>
   well_formed_prog lt \<Longrightarrow>
   unat pc < length lt \<and> unat pc \<ge> 0 \<Longrightarrow>
-  \<exists> num fst'. jit_fix_sem num prog xst = fst' \<and> match_state2 fst' (snd fxst')"
+  \<exists> num fst'. last_fix_sem num prog xst = fst' \<and> match_state2 fst' (snd fxst')"
 proof-
   assume a0:"flat_bpf_sem 1 (l_bin0,l_pc,l_jump) (pc,xst) = fxst'" and
   a1:"snd fxst' = Next xpc'' xrs'' xm'' xss''" and
@@ -370,8 +898,8 @@ proof-
                     done
                   done
                 
-                have "jit_fix_sem 2 prog' xst = x64_sem 2 prog' xst" using jit_fix_sem_def by simp
-                hence e0_0:"jit_fix_sem 2 prog' xst =  (
+                have "last_fix_sem 2 prog' xst = x64_sem 2 prog' xst" using last_fix_sem_def by simp
+                hence e0_0:"last_fix_sem 2 prog' xst =  (
                   case x64_decode xpc prog' of
                   None \<Rightarrow> Stuck |
                   Some (sz, ins) \<Rightarrow>
@@ -385,14 +913,14 @@ proof-
                   have e0:"x64_decode xpc prog' = x64_decode xpc l_bin0" 
                   proof(rule ccontr)*)
 
-                hence e1:"jit_fix_sem 2 prog' xst =  (
+                hence e1:"last_fix_sem 2 prog' xst =  (
                   case x64_decode xpc prog' of
                   Some (sz, Pcmpq_rr src dst) \<Rightarrow>
                     x64_sem 1 prog' (exec_instr (Pcmpq_rr src dst) sz xpc xrs xm xss)
                 )" using c0_0 a3 e0_0 apply(cases "x64_decode xpc prog'",simp_all) sorry
                 
-                have "jit_fix_sem 2 prog xst = x64_sem 2 prog xst" using jit_fix_sem_def by simp
-                hence e0:"jit_fix_sem 2 prog xst =  (
+                have "last_fix_sem 2 prog xst = x64_sem 2 prog xst" using last_fix_sem_def by simp
+                hence e0:"last_fix_sem 2 prog xst =  (
                   case x64_decode xpc prog of
                   None \<Rightarrow> Stuck |
                   Some (sz, ins) \<Rightarrow>
@@ -400,9 +928,9 @@ proof-
                 )"
                   by (metis Suc_1 a3 x64_sem.simps(3)) 
                 have e1:"\<exists> num src dst. x64_decode xpc prog = Some(num, Pcmpq_rr src dst)" sorry
-                hence "\<exists> src dst sz. jit_fix_sem 2 prog xst = x64_sem 1 prog (exec_instr (Pcmpq_rr src dst) sz xpc xrs xm xss)"
+                hence "\<exists> src dst sz. last_fix_sem 2 prog xst = x64_sem 1 prog (exec_instr (Pcmpq_rr src dst) sz xpc xrs xm xss)"
                   using e0 e1 by force
-                then obtain src dst sz where e2:"jit_fix_sem 2 prog xst = x64_sem 1 prog (exec_instr (Pcmpq_rr src dst) sz xpc xrs xm xss)" by auto
+                then obtain src dst sz where e2:"last_fix_sem 2 prog xst = x64_sem 1 prog (exec_instr (Pcmpq_rr src dst) sz xpc xrs xm xss)" by auto
                 hence e3:"sz = 3" using x64_encode_decode_consistency x64_encode_def list_in_list_prop sorry
 
               then show ?thesis sorry
@@ -465,8 +993,8 @@ proof-
               done
             done
           done
-        have b1:"jit_fix_sem (snd (l_pc!(unat pc))) prog xst = x64_sem (snd (l_pc!(unat pc))) prog xst" 
-          using jit_fix_sem_def by auto
+        have b1:"last_fix_sem (snd (l_pc!(unat pc))) prog xst = x64_sem (snd (l_pc!(unat pc))) prog xst" 
+          using last_fix_sem_def by auto
         have "\<exists> l. list_in_list l xpc l_bin0 \<longrightarrow> list_in_list l xpc prog" using jit_fix_not_change b0_1 a2 b0_0
           using list_in_list.simps(1) by metis
         then obtain l where b2:"list_in_list l xpc l_bin0 \<longrightarrow> list_in_list l xpc prog" by auto
@@ -477,9 +1005,9 @@ proof-
           (*have "x64_decode 0 l = x64_decode xpc l_bin0 \<and> x64_decode 0 l = x64_decode xpc prog" using list_in_list_x64_decode b0_2 sorry
           hence "x64_decode xpc l_bin0 = x64_decode xpc prog " using list_in_list_x64_decode by argo *)
           have "x64_bin_is_sequential (length l) l 0" sorry
-          hence "(jit_fix_sem (snd (l_pc!(unat pc))) prog xst) = (snd fxst')" 
+          hence "(last_fix_sem (snd (l_pc!(unat pc))) prog xst) = (snd fxst')" 
           using b0 b1 list_in_list_prop4 a1 by (metis True a3 b2)  
-        hence "\<exists> num fst'. num = (snd (l_pc!(unat pc))) \<and> jit_fix_sem num prog xst = fst' \<and> match_state2 fst' (snd fxst')"
+        hence "\<exists> num fst'. num = (snd (l_pc!(unat pc))) \<and> last_fix_sem num prog xst = fst' \<and> match_state2 fst' (snd fxst')"
           apply(unfold match_state2_def,simp_all) using a1 a3
           by(cases "snd fxst'",simp_all)           
         then show ?thesis by blast
@@ -492,139 +1020,8 @@ proof-
   qed
 qed
 
-(*(l_bin0,l_pc,l_jump) *)
-lemma n_steps_equiv_layer2:
-  "flat_bpf_sem n (l_bin0,l_pc,l_jump) (pc,xst) = fxst' \<Longrightarrow>
-  xst = Next xpc xrs xm xss \<Longrightarrow>
-  snd fxst' = Next xpc'' xrs'' xm'' xss'' \<Longrightarrow>
-  jitfix l_jump l_bin0 l_pc = Some prog \<Longrightarrow>
-  jitflat_bpf lt init_second_layer = (l_bin0,l_pc,l_jump) \<Longrightarrow>
-  well_formed_prog lt \<Longrightarrow>
-  \<exists> num fst'. jit_fix_sem num prog xst = fst' \<and> match_state2 fst' (snd fxst')"
-proof(induct n arbitrary:l_bin0 l_pc l_jump pc xst fxst' xpc xrs xm xss xpc'' xrs'' xm'' xss'' prog lt)
-  case 0 
-  assume assm0:"flat_bpf_sem 0 (l_bin0,l_pc,l_jump) (pc,xst) = fxst'" and
-    assm1:"xst = Next xpc xrs xm xss" and
-    assm2:"snd fxst' = Next xpc'' xrs'' xm'' xss''" and
-    assm3:"jitfix l_jump l_bin0 l_pc = Some prog" and
-    assm4:"jitflat_bpf lt init_second_layer = (l_bin0,l_pc,l_jump)" and
-    assm5:"well_formed_prog lt" 
-  have a0:"jit_fix_sem 0 prog xst = xst"  by (simp add: jit_fix_sem_def) 
-  have a1:"snd (flat_bpf_sem 0 (l_bin0,l_pc,l_jump) (pc,xst)) = xst" by simp
-
-  have "\<exists> num fst'. num = 0 \<and> jit_fix_sem num prog xst = fst'" using a0 by blast
-
-  hence "\<exists> num fst'. num = 0 \<and> jit_fix_sem num prog xst = fst' \<and> match_state2 fst' (snd fxst')"
-  using a0 a1 apply(unfold match_state2_def jit_fix_sem_def,simp_all) 
-    using assm1 assm0 apply(cases fxst') 
-    subgoal for a b apply(cases fxst')
-      subgoal for aa ba apply(cases xst)
-        subgoal for x11 x12 x13 x14 apply(cases xst,simp_all)
-          subgoal for x11a by(cases b,simp_all)
-          done
-        apply(cases xst,simp_all)
-          done
-        done
-      done
-           
-  then show ?case by blast
-    (*by (smt (verit, ccfv_threshold) flat_bpf_sem.simps(1) jit_fix_sem_def match_state2_def outcome.simps(4) snd_conv x64_sem.simps(1))*) 
-next
-  case (Suc n)
-  assume assm0:"flat_bpf_sem (Suc n) (l_bin0,l_pc,l_jump) (pc,xst) = fxst'" and
-    assm1:"xst = Next xpc xrs xm xss" and
-    assm2:"snd fxst' = Next xpc'' xrs'' xm'' xss''" and
-    assm3:"jitfix l_jump l_bin0 l_pc = Some prog"
-  have "\<exists> next_f. flat_bpf_sem 1 (l_bin0,l_pc,l_jump) (pc,xst) = next_f" by blast
-  then obtain next_f where b0:"flat_bpf_sem 1 (l_bin0,l_pc,l_jump) (pc,xst) = next_f" by auto
-  have "unat pc < length lt \<and> unat pc \<ge> 0" 
-  proof(rule ccontr)
-    assume assm:"\<not> (unat pc < length lt \<and> unat pc \<ge> 0)"
-    have "snd next_f = snd (let pair = flat_bpf_one_step (l_bin0,l_pc,l_jump) (pc, xst) in
-    flat_bpf_sem 0 (l_bin0,l_pc,l_jump) pair)" 
-      using b0 by fastforce
-    hence "snd next_f = snd (flat_bpf_one_step (l_bin0,l_pc,l_jump) (pc, xst))"
-      by (metis flat_bpf_sem.simps(1) prod.collapse) 
-    hence "snd next_f = Stuck" 
-      using flat_bpf_one_step_def assm assm2 apply(cases xst,simp_all)
-      subgoal for x11 x12 x13 x14 apply(cases "(l_bin0,l_pc,l_jump)",simp_all)
-        subgoal for a 
-          by (smt (z3) Suc.prems(5) add.right_neutral init_second_layer_def l_pc_length_prop list.size(3) nat_le_linear nat_less_le)
-        done
-      done
-      thus "False" using assm2
-        by (metis assm0 b0 err_is_still_err3 flat_bpf_sem_induct_aux2 outcome.distinct(1) prod.collapse) 
-  qed
-
-  hence "\<exists> num next_s. jit_fix_sem num prog xst = next_s \<and> match_state2 next_s (snd next_f)"
-    using one_steps_equiv_layer2 b0 assm0 assm2 assm3 flat_bpf_sem_induct_aux2 intermediate_step_is_ok3
-    by (metis (no_types, lifting) One_nat_def Suc.prems(2) Suc.prems(5) Suc.prems(6) less_eq_nat.simps(1) old.prod.exhaust snd_conv)  
-  then obtain num next_s where b1:"jit_fix_sem num prog xst = next_s \<and> match_state2 next_s (snd next_f)" by auto
-  have "\<exists> xpc' xrs' xm' xss'. snd next_f = Next xpc' xrs' xm' xss'"
-    by (metis Suc.prems(3) assm0 b0 flat_bpf_sem_induct_aux2 intermediate_step_is_ok3 less_eq_nat.simps(1) outcome.distinct(1) prod.collapse)
-  then obtain xpc' xrs' xm' xss' where b2:"snd next_f = Next xpc' xrs' xm' xss'" by auto
-  have b3:"flat_bpf_sem n (l_bin0,l_pc,l_jump) next_f = fxst'" using flat_bpf_sem_induct_aux2 b0 assm0 by blast 
-  have "flat_bpf_sem n (l_bin0, l_pc, l_jump) (pc, xst) = fxst' \<Longrightarrow>
-      xst = Next xpc xrs xm xss \<Longrightarrow> 
-      snd fxst' = Next xpc'' xrs'' xm'' xss'' \<Longrightarrow> 
-      jitfix l_jump l_bin0 l_pc = Some prog \<Longrightarrow> 
-      \<exists>(num::nat) fst'::outcome. jit_fix_sem num prog xst = fst' \<and> match_state2 fst' (snd fxst')" using Suc by simp
-  hence "\<exists>(num::nat) fst'::outcome. jit_fix_sem num prog (snd next_f) = fst' \<and> match_state2 fst' (snd fxst')" 
-    using b2 b1 match_state2_def assm3 b0 assm2 b3
-    by (metis Suc.hyps Suc.prems(5) Suc.prems(6) prod.collapse) 
-    
-  then show ?case
-    by (metis Suc.prems(2) b1 jit_fix_sem_def match_state2_def x64_sem_add) 
-qed
+*)
 
 
-lemma n_steps_equiv:
-  assumes assm0:"perir_sem n lt (pc,xxst) = xxst'" and
-  assm1:"xxst = Next xpc xrs xm xss" and
-  assm2:"snd xxst' = Next xpc' xrs' xm' xss'" and
-  assm3:"JITFlattern_def.match_state (pc,xxst) (pc,fxst)" and
-  assm4:"lt \<noteq> []" and
-  assm5:"well_formed_prog lt"and
 
-  assm6:"jitflat_bpf lt init_second_layer = (l_bin0,l_pc,l_jump)" and
-  assm7:"flat_bpf_sem n (l_bin0,l_pc,l_jump) (pc,fxst) = fxst'" and
-  assm8:"snd fxst' = Next xpc'' xrs'' xm'' xss''" and
-
-  assm9:"jitfix l_jump l_bin0 l_pc = Some prog" and
-  (*assm10:"jit_fix_sem n prog xst = fst'" and*)
-  assm11:"jitper insns = Some lt"
-  shows "\<exists> num fst'. jit_fix_sem num prog fxst = fst' \<and> match_state1 fst' (snd xxst')"
-proof-
-  have b0:"JITFlattern_def.match_state xxst' fxst'" 
-    using n_steps_equiv_layer1 assm3 assm0 assm1 assm2 assm4 assm5 assm11 assm6 assm7 assm8 by auto 
-  have "\<exists> xpc1 xrs xm xss. fxst = Next xpc1 xrs xm xss" 
-    using JITFlattern_def.match_state_def assm1 assm3 
-    apply(cases xxst,simp_all) 
-    apply(cases fxst,simp_all)
-    done
-  then obtain xpc1 xrs xm xss where b1:"fxst = Next xpc1 xrs xm xss" by auto
-  have b2:"\<exists> num fst'. jit_fix_sem num prog fxst = fst' \<and> match_state2 fst' (snd fxst')" 
-    using n_steps_equiv_layer2 assm7 assm9 b1 assm8 assm6 assm5 by blast
-  then obtain num fst' where b3:"jit_fix_sem num prog fxst = fst' \<and> match_state2 fst' (snd fxst')" by auto
-  hence b4:"match_state1 fst' (snd xxst')"
-    apply(unfold JITFlattern_def.match_state_def match_state2_def,simp_all)
-    using assm2 assm8 b0 b3
-    apply(cases fst',simp_all)
-    apply(cases "snd fxst'",simp_all)
-    apply(cases "snd xxst'",simp_all) 
-    subgoal for x11 x11a 
-      apply(cases "snd fxst'",simp_all)
-      subgoal for x11b
-        apply(unfold JITFlattern_def.match_state_def match_state2_def match_state1_def,simp_all)
-        apply(cases xxst',simp_all)
-        subgoal for a b 
-          apply(cases fxst',simp_all)
-          done
-        done
-      done
-    done
-  have "\<exists> num fst'. jit_fix_sem num prog fxst = fst' \<and> match_state1 fst' (snd xxst')" using b2 b4 b3 by blast
-  thus ?thesis using b2 by auto
-qed
-       
 end
