theory/JITFix_def.thy
@@ -66,7 +66,7 @@ definition fix_bpf_one_step :: "flat_bpf_prog \<Rightarrow> outcome \<Rightarrow
                 let ss' = update_stack caller fp (of_nat xpc) ss in
                   (case ss' of None \<Rightarrow> Stuck | 
                   Some ra \<Rightarrow> (Next (nat (fst (l_pc!(unat npc)))) rs' m ra))))  |
-                  Some(_, Pcmpq_rr src dst) \<Rightarrow> \<comment>\<open> TODO: if the first byte is the opcode of cmp? \<close>
+                  Some(_, Pjcc cond d) \<Rightarrow> \<comment>\<open> TODO: if the first byte is the opcode of cmp? \<close>
                           \<comment>\<open> case: BPF JMP \<close>
                           (case x64_sem num l_bin (Next xpc rs m ss) of
                           Stuck \<Rightarrow> Stuck | \<comment>\<open> if one step error, stop, it should be impossible \<close>
@@ -190,19 +190,170 @@ fun fix_bpf_sem :: "nat \<Rightarrow> flat_bpf_prog \<Rightarrow> outcome \<Righ
     fix_bpf_sem n lt pair
 )"
 
-(*
+
 definition match_state2::"outcome \<Rightarrow> outcome \<Rightarrow> bool" where
   "match_state2 fxst xxst \<equiv> 
   fxst = xxst \<and> (fxst \<noteq> Stuck \<or> xxst \<noteq> Stuck)"
-*)
 
-definition match_state2::"outcome \<Rightarrow> outcome \<Rightarrow> bool" where
+
+(*definition match_state2::"outcome \<Rightarrow> outcome \<Rightarrow> bool" where
   "match_state2 fxst xxst \<equiv> 
   (case fxst of (Next xpc xrs xm xss) \<Rightarrow>
     (case xxst of (Next xpc1 xrs1 xm1 xss1) \<Rightarrow> 
     xpc = xpc1 \<and> xrs = xrs1 \<and> match_mem xm xm1 \<and> xss = xss1 |
                    _ \<Rightarrow> False)|
                  _ \<Rightarrow> False)"
+*)
 
+
+value "x64_encode (Pcall_i 0x1111)"
+
+value "u8_list_of_i32 0x1111"
+
+value "x64_encode (Pjcc Cond_e 0x00000000)"
+
+value "u8_list_of_i32 0x11110000"
+
+value "u32_of_u8_list [0,0,0,0]"
+
+fun x64_bin_update ::"nat \<Rightarrow> x64_bin \<Rightarrow> nat \<Rightarrow> u8 list \<Rightarrow> x64_bin " where
+  "x64_bin_update 0 l _ _ = l" |
+  "x64_bin_update (Suc n) l pc u8_list =  (let l' = list_update l pc (hd u8_list) in x64_bin_update n l' (pc+1) (tl u8_list))"
+
+value "x64_bin_update 4 [232::8 word, 0::8 word, 0::8 word, 0::8 word, 0::8 word] 1 [17::8 word, 17::8 word, 0::8 word, 0::8 word]"
+
+value "x64_bin_update 4 [15::8 word, 132::8 word, 0::8 word, 0::8 word, 17::8 word, 17::8 word] 2 [0::8 word, 0::8 word, 17::8 word, 17::8 word]"
+(*
+definition get_updated_l_bin::"(int\<times>u64) \<Rightarrow> x64_bin \<Rightarrow> (int \<times> nat) list \<Rightarrow> x64_bin option"where
+  "get_updated_l_bin x l l_pc \<equiv> 
+    (let fix_begin_addr = fst (l_pc!(nat(fst x))); 
+        (target_begin_addr,num2) = l_pc!(unat (snd x)) in 
+        (case x64_decode (nat fix_begin_addr) l of 
+              Some(sz, Pcall_i _) \<Rightarrow> let offset = ((of_int target_begin_addr)::i32) - ((of_int fix_begin_addr+of_nat sz+1)::i32) in 
+                                     let u8_list = x64_encode (Pcall_i (ucast offset)) in
+                                     Some (x64_bin_update (length u8_list) l (nat fix_begin_addr) u8_list) |
+              Some(sz, Pcmpq_rr src dst) \<Rightarrow> let loc = nat fix_begin_addr+sz in 
+                    (case x64_decode loc l of 
+                            Some(sz2, Pjcc cond _) \<Rightarrow> let offset = ((of_int target_begin_addr)::i32) - ((of_nat (loc+sz2)+1)::i32) in
+                                                      let u8_list = x64_encode (Pjcc cond (ucast offset)) in                                                     
+                                                      Some (x64_bin_update (length u8_list) l loc u8_list) | 
+                            _ \<Rightarrow> None ) |
+              _ \<Rightarrow> None ))"
+*)
+
+definition get_updated_l_bin::"(int\<times>u64) \<Rightarrow> x64_bin \<Rightarrow> (int \<times> nat) list \<Rightarrow> x64_bin option"where
+  "get_updated_l_bin x l l_pc \<equiv> 
+    (let fix_begin_addr = fst (l_pc!(nat(fst x))); 
+        (target_begin_addr,num2) = l_pc!(unat (snd x)) in 
+        (case x64_decode (nat fix_begin_addr) l of 
+              Some(sz, Pcall_i _) \<Rightarrow> let u8_list = x64_encode (Pcall_i (of_int target_begin_addr)) in
+                                     Some (x64_bin_update (length u8_list) l (nat fix_begin_addr) u8_list) |
+              Some(sz, Pcmpq_rr src dst) \<Rightarrow> let loc = nat fix_begin_addr+sz in 
+                    (case x64_decode loc l of 
+                            Some(sz2, Pjcc cond _) \<Rightarrow> let offset = ((of_int target_begin_addr)::i32) - ((of_nat (loc+sz2)+1)::i32) in
+                                                      let u8_list = x64_encode (Pjcc cond (ucast offset)) in                                                     
+                                                      Some (x64_bin_update (length u8_list) l loc u8_list) | 
+                            _ \<Rightarrow> None ) |
+              _ \<Rightarrow> None ))"
+
+value "x64_decode 0 [72::8 word, 57::8 word, 195::8 word] "
+
+
+value "x64_decode 0 [15::8 word, 132::8 word, 0::8 word, 0::8 word, 0::8 word, 0::8 word] "
+
+
+value "get_updated_l_bin (0,1) [72::8 word, 57::8 word, 195::8 word, 15::8 word, 132::8 word, 0::8 word, 0::8 word, 0::8 word, 0::8 word ,195::8 word] [(0::int, 8::nat), (9::int, 1::nat)]"
+
+value "get_updated_l_bin (0,1) [232::8 word, 0::8 word, 0::8 word, 0::8 word, 0::8 word ,195::8 word] [(0::int, 1::nat), (6::int, 1::nat)]"
+
+(*input: l_jump x64_bin l_pc*)
+fun jitfix :: "((int\<times>u64) list) \<Rightarrow> x64_bin \<Rightarrow> (int \<times> nat) list \<Rightarrow> x64_bin option" where
+  "jitfix [] l _  = Some l" |
+  "jitfix (x#xs) l l_pc = (if l = [] then None else 
+    let res = get_updated_l_bin x l l_pc in case res of None \<Rightarrow> None | 
+                                                        Some l' \<Rightarrow> jitfix xs l' l_pc)"
+
+value "x64_encode (Pcmpq_rr RAX RBX)"
+
+value "x64_encode (Pret)"
+
+value "jitflat_bpf [(1, 1, [0x48,0x01,0xD8]),(1, 2, [0x48, 0x39, 0xc3, 0x0f, 0x84, 0x00, 0x00, 0x00, 0x00]), (1, 1, [0x48,0x01,0xD8]), (1, 1, [0x48,0x01,0xD8])] init_second_layer"
+
+value "jitfix [(1::int, 3::64 word)] [72::8 word, 1::8 word, 216::8 word, 72::8 word, 57::8 word, 195::8 word, 15::8 word, 132::8 word, 0::8 word, 0::8 word, 0::8 word, 0::8 word, 72::8 word, 1::8 word, 216::8 word, 72::8 word, 1::8 word, 216::8 word] [(0::int, 1::nat), (3::int, 1::nat), (12::int, 1::nat), (15::int, 1::nat)]"
+
+value "jitflat_bpf [(1, 2, [0x48, 0x39, 0xc3, 0x0f, 0x84, 0x00, 0x00, 0x00, 0x00]), (1, 1, [0xc3]), (1, 1, [0x48,0x01,0xD8]), (1, 1, [0x48,0x01,0xD8]),(1, -3, [0x48, 0x39, 0xc3, 0x0f, 0x84, 0x00, 0x00, 0x00, 0x00])] init_second_layer"
+
+value "jitfix [(0::int, 2::64 word), (4::int, 1::64 word)] [72::8 word, 57::8 word, 195::8 word, 15::8 word, 132::8 word, 0::8 word, 0::8 word, 0::8 word, 0::8 word, 195::8 word, 72::8 word, 1::8 word, 216::8 word, 72::8 word, 1::8 word, 216::8 word, 72::8 word, 57::8 word, 195::8 word,
+   15::8 word, 132::8 word, 0::8 word, 0::8 word, 0::8 word, 0::8 word] [(0::int, 1::nat), (9::int, 1::nat), (10::int, 1::nat), (13::int, 1::nat), (16::int, 1::nat)]"
+
+value "hd ([]::nat list)"
+value "tl ([]::nat list)"
+(*
+
+definition x64_bin_update ::"x64_bin \<Rightarrow> nat \<Rightarrow> u8 list \<Rightarrow> x64_bin " where
+ "x64_bin_update l pc u8_list \<equiv>  ( let l1 = list_update l pc (u8_list!0);
+                                       l2 = list_update l1 (pc+1) (u8_list!1);
+                                       l3 = list_update l2 (pc+2) (u8_list!2);   
+                                       l4 = list_update l3 (pc+3) (u8_list!3) in l4)"
+
+definition get_updated_l_bin::"(int\<times>u64) \<Rightarrow> x64_bin \<Rightarrow> (int \<times> nat) list \<Rightarrow> x64_bin"where
+  "get_updated_l_bin x l l_pc \<equiv> 
+    (let fix_begin_addr = fst (l_pc!(nat(fst x))); 
+        (target_begin_addr,num2) = l_pc!(unat (snd x)) in 
+        (case x64_decode (nat fix_begin_addr) l of 
+              Some(_, Pcall_i _) \<Rightarrow> let offset = ((of_int target_begin_addr)::i32) - ((of_int fix_begin_addr+5+1)::i32);
+                              u8_list = u8_list_of_i32 offset in
+                              x64_bin_update l (nat (fix_begin_addr+1)) u8_list | 
+              _ \<Rightarrow> let offset = ((of_int target_begin_addr)::i32) - ((of_int fix_begin_addr+3+6+1)::i32);
+                              u8_list = u8_list_of_i32 offset in                                                     
+                             x64_bin_update l (nat (fix_begin_addr+3+2)) u8_list))"*)
+
+
+
+(*definition update_l_jump_further::"flat_bpf_prog \<Rightarrow> hybrid_state \<Rightarrow> (hybrid_state \<times> flat_bpf_prog)" where
+ "update_l_jump_further lp st = (
+  let (l_bin,l_pc,l_jump) = lp in
+  let (pc, xst) = st in
+    (case xst of
+    Stuck \<Rightarrow> ((pc, Stuck), lp) |
+    Next xpc rs m ss \<Rightarrow> (
+    if unat pc \<ge> length l_pc \<or> unat pc < 0 then ((pc, Stuck), lp) else 
+    let num = snd (l_pc!(unat pc)) in 
+    let old_xpc = nat (fst (l_pc!(unat pc))) in 
+      if xpc \<noteq> old_xpc then ((pc, Stuck), lp) else 
+        if (\<exists> d. x64_decode xpc l_bin = Some(5, Pcall_i d)) then
+            (case find_target_pc_in_l_pc l_jump (uint pc) of 
+              None \<Rightarrow> ((pc, Stuck), lp) |
+              Some npc \<Rightarrow> 
+                (let caller = save_x64_caller rs; fp = save_x64_frame_pointer rs; 
+                    rs' = upate_x64_stack_pointer rs (stack_pointer ss) in
+                let ss' = update_stack caller fp (pc+1) ss in
+                  (case ss' of None \<Rightarrow> ((pc, Stuck), lp) | 
+                  Some ra \<Rightarrow> ((npc, (Next (nat (fst (l_pc!(unat npc)))) rs' m ra)), lp))))
+        else if (\<exists> src dst. x64_decode xpc l_bin = Some(3, Pcmpq_rr src dst)) then \<comment>\<open> TODO: if the first byte is the opcode of cmp? \<close>
+          \<comment>\<open> case: BPF JMP \<close>
+          (case x64_sem num l_bin (Next xpc rs m ss) of
+          Stuck \<Rightarrow> ((pc, Stuck), lp) | \<comment>\<open> if one step error, stop, it should be impossible \<close>
+          Next xpc1 rs1 m1 ss1 \<Rightarrow> (
+            if rs1 (CR ZF) = 1 then \<comment>\<open> must JUMP \<close>
+              (case find_target_pc_in_l_pc l_jump (uint pc) of
+              None \<Rightarrow> ((pc, Stuck), lp) |
+              Some npc \<Rightarrow>
+                ((npc, (Next (nat (fst (l_pc!(unat npc)))) rs1 m1 ss1)),lp)) \<comment>\<open> go to the target address in the jited x64 binary \<close>
+            else \<comment>\<open> donot JUMP \<close>
+              ((pc+1, (Next xpc1 rs1 m1 ss1)), lp)
+          ))
+        else if x64_decode xpc l_bin = Some(1,Pret) then
+          let (pc', ss', caller,fp) = update_stack2 ss in 
+          let rs' = restore_x64_caller rs caller fp in ((pc', Next xpc rs' m ss'), lp)
+          \<comment>\<open> case: NOT BPF JMP \<close>
+        else
+          ((pc+1, x64_sem num l_bin (Next xpc rs m ss)), lp)
+)))"
+*)
+
+
+definition last_fix_sem::"nat \<Rightarrow> x64_bin \<Rightarrow> outcome \<Rightarrow> outcome" where
+  "last_fix_sem n lt xst = x64_sem n lt xst"
 
 end
